Debug.lean
@@ -1,12 +1,6 @@
-import Sodium.FFI.SecretStream
+import Sodium.FFI
 
-open Lean Sodium FFI SecretStream
+open Lean Sodium FFI
 
 def main : IO Unit := do
-  let τ ← init Unit
-  let key ← keygen (τ := τ)
-  let (st, header) ← streamInitPush key
-  let message1 : ByteVector 16 := ByteVector.replicate 16 65 -- 16 'A's
-  let additionalData : ByteVector 4 := ByteVector.replicate 4 68 -- 4 'D's
-  let cipher1 ← streamPush st message1 additionalData STREAM_TAG_MESSAGE
-  IO.println s!"✓ Encrypted message 1 (size: {cipher1.size} bytes, tag: MESSAGE)"
+  return
