Sodium/Crypto/Types.lean
@@ -71,29 +71,23 @@ theorem toOption_some_iff {a : α} : ∀ r : DecryptResult α, toOption r = some
 
 end DecryptResult
 
-structure Nonce (spec : Spec) [spec.HasValidShape `nonce] where
-  data : ByteVector spec[`nonce]
-  deriving BEq, ToJson, FromJson
+abbrev Nonce (spec : Spec) [spec.HasValidShape `nonce] :=
+  ByteVector spec[`nonce]
 
-structure Seed (τ : Sodium σ) (spec : Spec) [h : spec.HasValidShape `seed] where
-  data : SecureVector τ <| USize.ofNatLT spec[`seed] (by simp [h.shape_is_valid])
-  deriving BEq
+abbrev Salt (τ : Sodium σ) (spec : Spec) [h : spec.HasValidShape `salt] :=
+  SecureVector τ <| USize.ofNatLT spec[`salt] (by simp [h.shape_is_valid])
 
-structure SymmKey (τ : Sodium σ) (spec : Spec) [h : spec.HasValidShape `symmkey] where
-  data : SecureVector τ <| USize.ofNatLT spec[`symmkey] (by simp [h.shape_is_valid])
-  deriving BEq
+abbrev SymmKey (τ : Sodium σ) (spec : Spec) [h : spec.HasValidShape `symmkey] :=
+  SecureVector τ <| USize.ofNatLT spec[`symmkey] (by simp [h.shape_is_valid])
 
-structure SecretKey (τ : Sodium σ) (spec : Spec) [h : spec.HasValidShape `secretkey] where
-  data : SecureVector τ <| USize.ofNatLT spec[`secretkey] (by simp [h.shape_is_valid])
-  deriving BEq
+abbrev SecretKey (τ : Sodium σ) (spec : Spec) [h : spec.HasValidShape `secretkey] :=
+  SecureVector τ <| USize.ofNatLT spec[`secretkey] (by simp [h.shape_is_valid])
 
-structure PublicKey (spec : Spec) [spec.HasValidShape `publickey] where
-  data : ByteVector spec[`publickey]
-  deriving BEq, ToJson, FromJson
+abbrev PublicKey (spec : Spec) [spec.HasValidShape `publickey] :=
+  ByteVector spec[`publickey]
 
-structure SharedKey (τ : Sodium σ) (spec : Spec) [h : spec.HasValidShape `sharedkey] where
-  data : SecureVector τ <| USize.ofNatLT spec[`sharedkey] (by simp [h.shape_is_valid])
-  deriving BEq
+abbrev SharedKey (τ : Sodium σ) (spec : Spec) [h : spec.HasValidShape `sharedkey] :=
+  SecureVector τ <| USize.ofNatLT spec[`sharedkey] (by simp [h.shape_is_valid])
 
 structure KeyPair (τ : Sodium σ) (spec : Spec) [spec.HasValidShape `publickey] [spec.HasValidShape `secretkey] where
   pkey : PublicKey spec
@@ -103,52 +97,17 @@ structure Session (τ : Sodium σ) (spec : Spec) [spec.HasValidShape `symmkey] w
   rx : SymmKey τ spec
   tx : SymmKey τ spec
 
-structure Mac (spec : Spec) [spec.HasValidShape `mac] where
-  data : ByteVector spec[`mac]
-  deriving BEq, ToJson, FromJson
+abbrev Hash (spec : Spec) [spec.HasValidShape `hash] :=
+  ByteVector spec[`hash]
 
-structure Hash (spec : Spec) [spec.HasValidShape `minhash] [spec.HasValidShape `maxhash] where
-  size : Nat
-  data : ByteVector size
-  shapeOf_minhash_le_size : spec[`minhash] ≤ size
-  shapeOf_maxhash_ge_size : spec[`maxhash] ≥ size
-  deriving BEq
+abbrev Context (spec : Spec) [spec.HasValidShape `context] :=
+  ByteVector spec[`context]
 
-namespace Hash
+abbrev Header (spec : Spec) [spec.HasValidShape `header] :=
+  ByteVector spec[`header]
 
-variable {spec : Spec} [spec.HasValidShape `minhash] [spec.HasValidShape `maxhash]
-
-instance : ToJson (Hash spec) where
-  toJson hash := json% {
-    size : $hash.size,
-    data : $hash.data
-  }
-
-instance : FromJson (Hash spec) where
-  fromJson? json := do
-    let size ← json.getObjValAs? Nat "size"
-    let data ← json.getObjValAs? (ByteVector size) "data"
-    if h1 : spec[`minhash] ≤ size then
-      if h2 : spec[`maxhash] ≥ size then
-        return ⟨size, data, h1, h2⟩
-      else
-        throw "expected data size to be at most maxhash"
-    else
-      throw "expected data size to be at least minhash"
-
-end Hash
-
-structure Salt (τ : Sodium σ) (spec : Spec) [h : spec.HasValidShape `salt] where
-  data : SecureVector τ <| USize.ofNatLT spec[`salt] (by simp [h.shape_is_valid])
-  deriving BEq
-
-structure Context (spec : Spec) [spec.HasValidShape `context] where
-  data : ByteVector spec[`context]
-  deriving BEq, ToJson, FromJson
-
-structure Header (spec : Spec) [spec.HasValidShape `header] where
-  data : ByteVector spec[`header]
-  deriving BEq, ToJson, FromJson
+abbrev Signature (spec : Spec) [spec.HasValidShape `signature] :=
+  ByteVector spec[`signature]
 
 structure CipherText (spec : Spec) [spec.HasValidShape `nonce] [spec.HasValidShape `mac] where
   size : Nat
@@ -179,14 +138,14 @@ instance : FromJson (CipherText spec) where
 
 end CipherText
 
-structure SealedCipherText (spec : Spec) [spec.HasValidShape `seal] where
+structure SealedCipherText (spec : Spec) [spec.HasValidShape `publickey] [spec.HasValidShape `mac] where
   size : Nat
   data : ByteVector size
-  shapeOf_seal_le_size : spec[`seal] ≤ size
+  shapeOf_seal_le_size : spec[`publickey] + spec[`mac] ≤ size
 
 namespace SealedCipherText
 
-variable {spec : Spec} [spec.HasValidShape `seal]
+variable {spec : Spec} [spec.HasValidShape `publickey] [spec.HasValidShape `mac]
 
 instance : ToJson (SealedCipherText spec) where
   toJson cipher := json% {
@@ -198,7 +157,7 @@ instance : FromJson (SealedCipherText spec) where
   fromJson? json := do
     let size ← json.getObjValAs? Nat "size"
     let data ← json.getObjValAs? (ByteVector size) "data"
-    if h : spec.shapeOf `seal ≤ size then
+    if h : spec.shapeOf `publickey + spec.shapeOf `mac ≤ size then
       return ⟨size, data, h⟩
     else
       throw "expected data to contain embedded seal"
