Sodium/Data/Digest.lean
@@ -1,0 +1,69 @@
+import Sodium.Data.Chunk
+import Sodium.Crypto.Monad
+
+universe u v
+
+open Lean Sodium FFI GenericHash Crypto
+
+abbrev Digest := Hash Blake2b
+
+class ToDigest (α : Type u) where
+  digest : α → Digest
+
+export ToDigest (digest)
+
+namespace Digest
+
+variable {α : Type u} {β : Type v}
+
+def toName (dig : Digest) : Name := Name.str Blake2b.name dig.toBase64
+
+instance : Inhabited Digest where
+  default := GenericHash.hash default |>.cast
+
+instance [ToJson α] : ToDigest α where
+  digest x := GenericHash.hash (toJson x).compress.toUTF8 |>.cast (by native_decide)
+
+instance [ToChunks α] : ToDigest α where
+  digest x := Id.run do
+    let mut stream := hashInit
+    for chunk in toChunks x do
+      stream := hashUpdate stream chunk.compress.toUTF8
+    return hashFinal stream |>.cast
+
+instance : ToDigest Unit where
+  digest _ := digest (json% null)
+
+instance {n : Nat} : ToDigest (Fin n) where
+  digest x := digest (json% $x.toNat)
+
+instance [ToDigest α] [ToDigest β] : ToDigest (α × β) where
+  digest x := Id.run do
+    let mut stream := hashInit
+    stream := hashUpdate stream (digest x.1).toArray
+    stream := hashUpdate stream (digest x.2).toArray
+    return hashFinal stream |>.cast
+
+instance [ToDigest α] [ToDigest β] : ToDigest (α ⊕ β) where
+  digest x := Id.run do
+    let mut stream := hashInit
+    match x with
+    | .inl y =>
+      stream := hashUpdate stream (digest <| json% false).toArray
+      stream := hashUpdate stream (digest y).toArray
+    | .inr z =>
+      stream := hashUpdate stream (digest <| json% true).toArray
+      stream := hashUpdate stream (digest z).toArray
+    return hashFinal stream |>.cast
+
+end Digest
+
+class EqShape {α : Type u} {β : Type v} [ToDigest α] [ToDigest β] (a : α) (b : β) : Prop where
+  eq_shape : digest a = digest b
+
+namespace Lean.Name
+
+open Crypto in
+def blake2b {α : Type u} [ToDigest α] (x : α) : Name := Digest.toName (digest x)
+
+end Lean.Name
