Sodium/Data/Encodable/Basic.lean
@@ -1,0 +1,327 @@
+import Aesop
+import Sodium.Data.ByteArray
+
+open Lean
+
+universe u v
+
+namespace RBNode
+
+variable {α : Type u} [Ord α] [Std.ReflOrd α] {β : Type v}
+
+@[simp]
+theorem insert_find_eq_some : ∀ (k : α) (v : β), RBNode.find compare (RBNode.insert compare RBNode.leaf k v) k = some v := by
+  intro k v
+  unfold RBNode.insert RBNode.ins
+  split
+  . contradiction
+  . unfold RBNode.find
+    have : compare k k = .eq := by exact Std.compare_self
+    split <;> rename_i h
+    . rw [this] at h
+      contradiction
+    . rw [this] at h
+      contradiction
+    . rfl
+
+end RBNode
+
+namespace String
+
+instance instReflOrd : Std.ReflOrd String where
+  compare_self := by
+    intro s
+    unfold compare instOrdString compareOfLessAndEq
+    simp only [String.lt_irrefl, ↓reduceIte]
+
+end String
+
+namespace Json
+
+variable {α β : Json}
+
+@[simp]
+theorem num_getNat?_eq_ok : ∀ n, (Json.num (JsonNumber.fromNat n)).getNat? = .ok n := by
+  intro n
+  unfold Json.getNat? JsonNumber.fromNat
+  split
+  . rename_i m h
+    simp_all only [Int.ofNat_eq_coe, Json.num.injEq, JsonNumber.mk.injEq, and_true]
+    rw [← Int.mem_toNat?] at h
+    unfold Int.toNat? at h
+    simp at h
+    subst h
+    rfl
+  . rfl
+
+@[simp]
+theorem mkObj_getObjVal?_eq_ok : ∀ s, (Json.mkObj [(s, α)]).getObjVal? s = .ok α := by
+  intro s
+  unfold Json.mkObj Json.getObjVal?
+  simp only [Id.run, bind_pure_comp, map_pure, List.forIn_pure_yield_eq_foldl, List.foldl_cons,
+    List.foldl_nil, pure_bind, RBNode.insert_find_eq_some]
+  rfl
+
+@[simp]
+theorem arr_getArrVal?_0_eq_ok : (Json.arr #[α, β]).getArrVal? 0 = .ok α := by
+  unfold Json.getArrVal?
+  rfl
+
+@[simp]
+theorem arr_getArrVal?_1_eq_ok : (Json.arr #[α, β]).getArrVal? 1 = .ok β := by
+  unfold Json.getArrVal?
+  rfl
+
+end Json
+
+class Encodable (α : Type u) where
+  encode : α → Json
+  decode? : Json → Option α
+  encodek : ∀ a, decode? (encode a) = some a
+
+export Encodable (encode decode?)
+
+attribute [simp] Encodable.encodek
+
+class LawfulJson (α : Type u) [ToJson α] [FromJson α] where
+  jsonk : ∀ a, fromJson? (α := α) (toJson a) = .ok a
+
+instance {α : Type u} [ToJson α] [FromJson α] [h : LawfulJson α] : Encodable α where
+  encode := toJson
+  decode? x := fromJson? x |>.toOption
+  encodek := by
+    intro a
+    obtain ⟨jsonk⟩ := h
+    specialize jsonk a
+    simp_all only
+    rfl
+
+instance {α : Type u} [Encodable α] : ToJson α := ⟨encode⟩
+
+instance {α : Type u} [TypeName α] [Encodable α] : FromJson α where
+  fromJson? json := decode? (α := α) json |>.getDM (throw (TypeName.typeName α).toString)
+
+private instance {α : Type u} [Encodable α] : FromJson α :=
+  ⟨fun json => decode? (α := α) json |>.getDM (throw default)⟩
+
+instance {α : Type u} [Encodable α] : LawfulJson α where
+  jsonk _ := by
+    simp [fromJson?, toJson]
+    rfl
+
+namespace Encodable
+
+open Encodable (encodek)
+
+variable {α : Type u} {β : Type v} [Encodable α]
+
+def withErrorMsg (msg : String) (inst : Encodable β) : FromJson β where
+  fromJson? json := decode? (α := β) json |>.getDM (throw msg)
+
+@[simp]
+theorem decode?_encode_eq : decode? ∘ encode (α := α) = some := by
+  funext x
+  simp only [Function.comp_apply, encodek]
+
+theorem encode_inj : ∀ ⦃a b : α⦄, encode a = encode b → a = b
+  | x, y, h => Option.some.inj (by rw [← encodek, h, encodek])
+
+@[simp]
+theorem encode_eq_iff {a b : α} : encode a = encode b ↔ a = b :=
+  ⟨by exact @encode_inj _ _ _ _, congrArg encode⟩
+
+def ofLeftInj (f : β → α) (g : α → Option β) (h : ∀ x, g (f x) = some x) : Encodable β :=
+  ⟨fun b => encode (f b), fun json => (decode? json).bind g, by simp [encodek, h]⟩
+
+def ofEquiv (f : β → α) (g : α → β) (h : ∀ x, g (f x) = x) : Encodable β :=
+  ⟨fun b => encode (f b), fun json => (decode? json).map g, by simp [encodek, h]⟩
+
+def _root_.Empty.encodable : Encodable Empty :=
+  ⟨Empty.elim, fun _ => none, fun x => Empty.elim x⟩
+
+instance _root_.Json.instEncodable : Encodable Json where
+  encode := id
+  decode? := pure
+  encodek _ := by rfl
+
+instance _root_.Nat.instEncodable : Encodable Nat where
+  encode n := json% $n
+  decode? json := json.getNat?.toOption
+  encodek _ := by rfl
+
+instance _root_.String.instEncodable : Encodable String where
+  encode s := json% $s
+  decode? json := json.getStr?.toOption
+  encodek _ := by rfl
+
+instance _root_.Bool.instEncodable : Encodable Bool where
+  encode | true => json% true | false => json% false
+  decode? json := fromJson? (α := Bool) json |>.toOption
+  encodek _ := by split <;> rfl
+
+instance _root_.Unit.instEncodable : Encodable Unit where
+  encode _ := json% null
+  decode? | json% null => some () | _ => none
+  encodek _ := by rfl
+
+instance _root_.Array.instEncodable : Encodable (Array α) where
+  encode xs := Json.arr (xs.map encode)
+  decode?
+    | .arr xs => xs.mapM decode?
+    | _ => none
+  encodek _ := by
+    simp [Array.mapM_map]
+    have : some (α := α) = fun x => pure (id x) := by rfl
+    rw [this, Array.mapM_pure]
+    simp only [Array.map_id_fun, id_eq, Option.pure_def]
+
+instance _root_.Fin.instEncodable {n : Nat} : Encodable (Fin n) where
+  encode x := json% $x.toNat
+  decode? json := do
+    let m ← json.getNat?.toOption
+    if h : m < n then some ⟨m, h⟩ else none
+  encodek _ := by
+    unfold Except.toOption
+    simp only [toJson, Fin.toNat_eq_val, Json.num_getNat?_eq_ok, Option.bind_eq_bind,
+      Option.bind_some, Fin.is_lt, ↓reduceDIte, Fin.eta]
+
+def _root_.Fin.encodable0 : Encodable (Fin 0) :=
+  have : Encodable Empty := by exact Empty.encodable
+  ofEquiv (α := Empty) Fin.elim0 Empty.elim (by exact fun x => Fin.elim0 x)
+
+instance _root_.UInt8.instEncodable : Encodable UInt8 :=
+  ofEquiv UInt8.toFin UInt8.ofFin (by exact fun _ => rfl)
+
+instance _root_.UInt16.instEncodable : Encodable UInt16 :=
+  ofEquiv UInt16.toFin UInt16.ofFin (by exact fun _ => rfl)
+
+instance _root_.UInt32.instEncodable : Encodable UInt32 :=
+  ofEquiv UInt32.toFin UInt32.ofFin (by exact fun _ => rfl)
+
+instance _root_.UInt64.instEncodable : Encodable UInt64 :=
+  ofEquiv UInt64.toFin UInt64.ofFin (by exact fun _ => rfl)
+
+private def _root_.ByteArray.encodeImpl : ByteArray → Json := ByteArray.toJson
+private def _root_.ByteArray.decode?Impl : Json → Option ByteArray := Except.toOption ∘ ByteArray.fromJson?
+
+@[implemented_by ByteArray.encodeImpl]
+def _root_.ByteArray.encode (bs : ByteArray) : Json := Encodable.encode bs.data
+
+@[implemented_by ByteArray.decode?Impl]
+def _root_.ByteArray.decode? (json : Json) : Option ByteArray := do
+  let bs ← Encodable.decode? (α := Array UInt8) json
+  return ⟨bs⟩
+
+instance _root_.ByteArray.instEncodable : Encodable ByteArray where
+  encode := ByteArray.encode
+  decode? := ByteArray.decode?
+  encodek _ := by
+    unfold ByteArray.decode? ByteArray.encode
+    simp only [encodek, Option.pure_def, Option.bind_eq_bind, Option.bind_some]
+
+instance _root_.Option.instEncodable : Encodable (Option α) where
+  encode
+    | none => json% null
+    | some x => json% { some: $(encode x) }
+  decode?
+    | json% null => some none
+    | json =>
+      match json.getObjVal? "some" with
+      | .error _ => none
+      | .ok json =>
+        match decode? (α := α) json with
+        | none => none
+        | some a => some (some a)
+  encodek o := by
+    cases o with
+    | some a =>
+      simp
+      split
+      . contradiction
+      . simp_all only [imp_false]
+        split
+        . contradiction
+        . rename_i json heq
+          simp [toJson] at heq
+          subst heq
+          simp only [encodek]
+    | none => rfl
+
+instance _root_.Sum.instEncodable [Encodable β] : Encodable (α ⊕ β) where
+  encode
+    | .inl a => json% { inl: $a }
+    | .inr b => json% { inr: $b }
+  decode? json :=
+    match json.getObjVal? "inl" with
+    | .ok json => decode? (α := α) json |>.map .inl
+    | .error _ =>
+      match json.getObjVal? "inr" with
+      | .ok json => decode? (α := β) json |>.map .inr
+      | .error _ => none
+  encodek a := by
+    cases a with
+    | inl _ =>
+      simp_all only [Json.mkObj_getObjVal?_eq_ok, Option.map_eq_some_iff, Sum.inl.injEq, exists_eq_right]
+      simp only [toJson, encodek]
+    | inr _ =>
+      simp_all only [Json.mkObj_getObjVal?_eq_ok]
+      split
+      . simp_all only [Option.map_eq_some_iff, reduceCtorEq, and_false, exists_false]
+        contradiction
+      . simp_all only [Option.map_eq_some_iff, Sum.inr.injEq, exists_eq_right]
+        simp only [toJson, encodek]
+
+instance _root_.Prod.instEncodable [Encodable β] : Encodable (α × β) where
+  encode x := json% [$(x.1), $(x.2)]
+  decode? json :=
+    match json.getArrVal? 0, json.getArrVal? 1 with
+    | .ok fst, .ok snd =>
+      (decode? (α := α) fst).bind fun a => (decode? (α := β) snd).bind fun b => some (a, b)
+    | _, _ => none
+  encodek a := by
+    obtain ⟨fst, snd⟩ := a
+    simp only [toJson, Json.arr_getArrVal?_0_eq_ok, Json.arr_getArrVal?_1_eq_ok, encodek,
+      Option.bind_some]
+
+instance _root_.String.Pos.instEncodable : Encodable String.Pos :=
+  ofEquiv (α := Nat) String.Pos.byteIdx String.Pos.mk (by exact fun _ => rfl)
+
+instance _root_.Substring.instEncodable : Encodable Substring :=
+  ofEquiv (α := String × String.Pos × String.Pos)
+    (fun x => ⟨x.str, x.startPos, x.stopPos⟩)
+    (fun x => ⟨x.1, x.2.1, x.2.2⟩)
+    (by exact fun _ => rfl)
+
+section Sigma
+
+variable {γ : α → Type v} [∀ a, Encodable (γ a)]
+
+instance _root_.Sigma.instEncodable : Encodable (Sigma γ) where
+  encode x := json% [$(x.1), $(x.2)]
+  decode? json :=
+    match json.getArrVal? 0, json.getArrVal? 1 with
+    | .ok fst, .ok snd =>
+      (decode? (α := α) fst).bind fun a => (decode? (α := γ a) snd).bind fun b => some ⟨a, b⟩
+    | _, _ => none
+  encodek a := by
+    obtain ⟨fst, snd⟩ := a
+    simp only [toJson, Json.arr_getArrVal?_0_eq_ok, Json.arr_getArrVal?_1_eq_ok, encodek,
+      Option.bind_some]
+
+end Sigma
+
+section Subtype
+
+variable {P : α → Prop} [DecidablePred P]
+
+instance _root_.Subtype.instEncodable : Encodable {a : α // P a} where
+  encode x := encode x.1
+  decode? json := (decode? (α := α) json).bind fun a => if h : P a then some ⟨a, h⟩ else none
+  encodek x := by
+    obtain ⟨_, h⟩ := x
+    simp only [encodek, Option.bind_some, Option.dite_none_right_eq_some, exists_prop, and_true]
+    exact h
+
+end Subtype
+
+end Encodable
