Sodium/Data/Encodable/Pi.lean
@@ -1,0 +1,54 @@
+import Sodium.Data.Encodable.Basic
+
+universe u
+
+namespace Vector
+
+variable {n : Nat} {α : Type u}
+
+instance instEncodable [Encodable α] : Encodable (Vector α n) where
+  encode x := encode x.toArray
+  decode? json := do
+    let x ← decode? (α := Array α) json
+    if h : x.size = n then some ⟨x, h⟩
+    else none
+  encodek _ := by
+    simp only [Encodable.encodek, Option.bind_eq_bind, Option.bind_some, size_toArray,
+      ↓reduceDIte, mk_toArray]
+
+theorem get_eq_get_toList (v : Vector α n) (i : Fin n) :
+    v.get i = v.toList.get (Fin.cast (by exact Eq.symm length_toList) i) :=
+  rfl
+
+@[simp]
+theorem get_ofFn {n} (f : Fin n → α) (i) : (ofFn f).get i = f i := by
+  simp [get_eq_get_toList]
+
+@[simp]
+theorem ofFn_get (v : Vector α n) : ofFn v.get = v := by
+  rcases v with ⟨l, rfl⟩
+  simp_all only [eq_mk, toArray_ofFn]
+  ext i hi₁ hi₂ : 1
+  · simp_all only [Array.size_ofFn]
+  · simp_all only [Array.getElem_ofFn]
+    rfl
+
+end Vector
+
+namespace Encodable
+
+variable {α : Type u}
+
+instance finArrow {n : Nat} [Encodable α] : Encodable (Fin n → α) :=
+  ofEquiv Vector.ofFn Vector.get fun x => by
+    funext y
+    exact Vector.get_ofFn x y
+
+instance finPi (n : Nat) (π : Fin n → Type u) [∀ i, Encodable (π i)] : Encodable (∀ i, π i) :=
+  ofEquiv
+    (α := {f : Fin n → Σ i, π i // ∀ i, (f i).1 = i})
+    (fun f => ⟨fun i => ⟨i, f i⟩, fun _ => rfl⟩)
+    (fun f i => by rw [← f.2 i]; exact (f.1 i).2)
+    (by simp only [eq_mpr_eq_cast, cast_eq, implies_true])
+
+end Encodable
