Sodium/Data/Encodable/WType.lean
@@ -1,0 +1,60 @@
+import Sodium.Data.Encodable.Pi
+
+universe u v w
+
+inductive WType {α : Type u} (β : α → Type v)
+  | mk (a : α) (f : β a → WType β) : WType β
+
+instance : Inhabited (WType fun _ : Unit => Empty) := ⟨WType.mk () Empty.elim⟩
+
+namespace WType
+
+variable {α : Type u} {β : α → Type v}
+
+def toSigma : WType β → Σ a : α, β a → WType β
+  | ⟨a, f⟩ => ⟨a, f⟩
+
+def ofSigma : (Σ a : α, β a → WType β) → WType β
+  | ⟨a, f⟩ => ⟨a, f⟩
+
+@[simp]
+theorem ofSigma_toSigma : ∀ w : WType β, ofSigma (toSigma w) = w
+  | ⟨_, _⟩ => rfl
+
+@[simp]
+theorem toSigma_ofSigma : ∀ s : Σ a : α, β a → WType β, toSigma (ofSigma s) = s
+  | ⟨_, _⟩ => rfl
+
+def elim (γ : Type w) (fγ : (Σ a, β a → γ) → γ) : WType β → γ
+  | ⟨a, f⟩ => fγ ⟨a, fun b => elim γ fγ (f b)⟩
+
+variable {ι : α → Nat}
+
+def depth : WType (fun a => Fin (ι a)) → Nat
+  | ⟨a, f⟩ =>
+    let n := ι a
+    if h : n ≠ 0 then
+      have : NeZero n := ⟨by exact h⟩
+      let ns := List.range n |>.map (Fin.ofNat n)
+      1 + ns.foldl (init := 0) fun acc i => max acc (depth (f i))
+    else 1
+
+theorem depth_pos (w : WType fun a => Fin (ι a)) : 0 < w.depth := by
+  obtain ⟨a, f⟩ := w
+  unfold depth
+  simp only [ne_eq, dite_not]
+  split
+  . trivial
+  . omega
+
+theorem depth_lt_depth_mk (a : α) (f : Fin (ι a) → WType fun i => Fin (ι i)) (i : Fin (ι a)) : depth (f i) < depth ⟨a, f⟩ := by
+  sorry
+
+end WType
+
+abbrev WFin {α : Type u} (ι : α → Nat) (n : Nat) :=
+  { w : WType fun a => Fin (ι a) // w.depth ≤ n }
+
+namespace WFin
+
+end WFin
