Sodium/Meta/Syntax.lean
@@ -1,0 +1,7 @@
+import Sodium.Data.Digest
+
+open Lean Meta Elab
+
+namespace Lean.Syntax
+
+end Lean.Syntax
